unify_types is idempotent and clean_tysubst

candle/overloading/syntax/holSyntaxExtraScript.sml
@@ -7472,6 +7472,76 @@ Proof
   >> fs[]
 QED
 
+Definition idempotent_def:
+  idempotent s = !ty. TYPE_SUBST s (TYPE_SUBST s ty) = TYPE_SUBST s ty
+End
+
+Theorem idempotent_NIL:
+  idempotent []
+Proof
+  fs[idempotent_def,TYPE_SUBST_NIL]
+QED
+
+Theorem idempotent_clean_tysubst:
+  !s. idempotent s =
+    !ty. TYPE_SUBST (clean_tysubst s) (TYPE_SUBST (clean_tysubst s) ty)
+      = TYPE_SUBST (clean_tysubst s) ty
+Proof
+  fs[idempotent_def,GSYM clean_tysubst_TYPE_SUBST_eq]
+QED
+
+Theorem idempotent_thm:
+  !s. idempotent s <=>
+    !x. MEM (Tyvar x) (MAP SND $ clean_tysubst s)
+    ==> ~MEM x (FLAT $ MAP tyvars $ MAP FST $ clean_tysubst s)
+Proof
+  fs[EQ_IMP_THM,idempotent_clean_tysubst]
+  >> rpt strip_tac
+  >- (
+    qmatch_asmsub_abbrev_tac `TYPE_SUBST s' _`
+    >> dxrule_then strip_assume_tac TYPE_SUBST_MEM_MAP_SND
+    >> Cases_on `MEM x (tyvars b)`
+    >- (
+      Cases_on `b` >- (
+        qspec_then `s` assume_tac clean_tysubst_ineq
+        >> gs[tyvars_def,EVERY_MEM,ELIM_UNCURRY] >> res_tac >> fs[]
+      )
+      >> fs[GSYM subtype_at_tyvars]
+      >> drule_then (qspec_then `s'` assume_tac) subtype_at_TYPE_SUBST
+      >> first_x_assum $ qspec_then `Tyvar x` assume_tac
+      >> gs[]
+    )
+    >> gvs[MEM_FLAT,MEM_MAP]
+    >> rev_dxrule_then strip_assume_tac $ cj 1 $ REWRITE_RULE[EQ_IMP_THM] $ GSYM subtype_at_tyvars
+    >> first_x_assum $ qspec_then `SND y'` assume_tac
+    >> `?a. SND y' = Tyvar a` by (
+      qunabbrev_tac `s'`
+      >> imp_res_tac $ Q.ISPEC `SND` MEM_MAP_f
+      >> imp_res_tac $ REWRITE_RULE[EVERY_MEM] clean_tysubst_SND_Tyvar
+      >> fs[ELIM_UNCURRY]
+    )
+    >> drule_then (qspec_then `s'` assume_tac) subtype_at_TYPE_SUBST
+    >> Cases_on `y'` >> gvs[]
+    >> dxrule_at Any TYPE_SUBST_MEM'
+    >> impl_keep_tac >- fs[Abbr`s'`,clean_tysubst_ALL_DISTINCT_MAP_SND] >> strip_tac
+    >> drule_all_then assume_tac TYPE_SUBST_MEM' >> gvs[]
+    >> qpat_x_assum `Tyvar _ = _` $ (fn x => fs[GSYM x,tyvars_def])
+  )
+  >> qmatch_goalsub_abbrev_tac `TYPE_SUBST s' _`
+  >> rw[TYPE_SUBST_tyvars,TYPE_SUBST_compose]
+  >> REWRITE_TAC $ map GSYM [TYPE_SUBST_compose,TYPE_SUBST_def]
+  >> reverse $ Cases_on `MEM (Tyvar x) (MAP SND s')`
+  >- fs[TYPE_SUBST_drop_all]
+  >> res_tac
+  >> dxrule_then strip_assume_tac TYPE_SUBST_MEM_MAP_SND >> fs[]
+  >> CONV_TAC $ LAND_CONV $ REWR_CONV $ GSYM TYPE_SUBST_NIL
+  >> rw[TYPE_SUBST_tyvars,REV_ASSOCD_def]
+  >> irule REV_ASSOCD_NOT_MEM_drop
+  >> first_x_assum $ match_mp_tac o ONCE_REWRITE_RULE[MONO_NOT_EQ]
+  >> rw[MEM_FLAT,MEM_MAP,PULL_EXISTS]
+  >> goal_assum drule >> fs[]
+QED
+
 Definition unify_types_invariant_def:
   unify_types_invariant orig_l l sigma =
     (* The substitution's domain is not in the worklist *)
@@ -7502,10 +7572,16 @@ Definition unify_types_invariant_def:
         (subtype_at (TYPE_SUBST sigma x) p = SOME a /\ subtype_at (TYPE_SUBST sigma y) p = SOME b)
         \/ (subtype_at (TYPE_SUBST sigma x) p = SOME b /\ subtype_at (TYPE_SUBST sigma y) p = SOME a)))
     (* If we have a certificate for two not unifiable types then the
-       original list could not have been unifiable *)
-    /\ (?s. EVERY (λ(x,y). TYPE_SUBST s x = TYPE_SUBST s y) orig_l
+       original list could not have been unifiable;
+       most general unifier *)
+    /\ (!s. EVERY (λ(x,y). TYPE_SUBST s x = TYPE_SUBST s y) orig_l
       ==> ?s'. EVERY (λ(x,y). (TYPE_SUBST s' o TYPE_SUBST sigma) x
-        = (TYPE_SUBST s' o TYPE_SUBST sigma) y) orig_l)
+        = (TYPE_SUBST s' o TYPE_SUBST sigma) y
+        /\ (TYPE_SUBST s' o TYPE_SUBST sigma) x = TYPE_SUBST s x
+        /\ (TYPE_SUBST s' o TYPE_SUBST sigma) y = TYPE_SUBST s y
+        ) orig_l)
+    /\ EVERY (UNCURRY $<>) sigma
+    /\ idempotent sigma
 (*    (* The substitution's domain is not work list *)
     /\ (!a. MEM (Tyvar a) (MAP SND sigma) ==>
          ~MEM a (FLAT(MAP (tyvars o FST) l)) /\ ~MEM a (FLAT(MAP (tyvars o SND) l)))
@@ -7554,7 +7630,6 @@ Proof
   fs (map (SIMP_RULE (srw_ss()) [IN_DEF]) [MEM_FOLDR_LIST_UNION,MEM_FLAT,MEM_MAP])
   \\ rw[EQ_IMP_THM] \\ metis_tac[]
 QED
-
 
 Theorem unify_types_invariant_pres2[local]:
   unify_types_invariant orig_l ((Tyapp a atys, Tyapp b btys)::l) sigma
@@ -7618,8 +7693,7 @@ Proof
   )
   >- (
     fs[unify_types_invariant_def]
-    >> asm_exists_tac
-    >> rw[]
+    >> goal_assum $ drule
   )
 QED
 
@@ -7845,47 +7919,108 @@ Proof
       >> fs[]
     )
   )
+  >> conj_tac
   >- (
-    fs[unify_types_invariant_def,EVERY_MEM,unifiable_def,ELIM_UNCURRY]
-    >> rw[EVERY_MEM,ELIM_UNCURRY,unifiable_def]
-    >> first_x_assum (qspecl_then [`Tyvar a`,`ty`] mp_tac)
-    >> rw[]
+    qx_gen_tac `s` >> strip_tac
+    >> fs[unify_types_invariant_def,EVERY_MEM,unifiable_def,ELIM_UNCURRY]
+    >> first_x_assum $ drule_then strip_assume_tac
+    >> qpat_x_assum `!a b. _ \/ _ ==> _` $ assume_tac o cj 1 o
+      Ho_Rewrite.REWRITE_RULE[FORALL_AND_THM,DISJ_IMP_THM,IMP_CONJ_THM]
+    >> fs[]
     >> qmatch_asmsub_abbrev_tac `subtype_at (TYPE_SUBST _ x) p = SOME in_x`
     >> qmatch_asmsub_abbrev_tac `subtype_at (TYPE_SUBST _ y) p = SOME in_y`
-    >> qexists_tac `s`
-    >> rw[]
-    >> fs[]
-    >> qexists_tac `s'`
-    >> rpt strip_tac
-    >> qpat_x_assum `!x. _` kall_tac
-    >> first_assum drule
-    >> first_x_assum (qspec_then `(x,y)` mp_tac)
-    >> rw[]
+    >> qmatch_asmsub_rename_tac `TYPE_SUBST s' $ TYPE_SUBST sigma _`
+    >> qexists_tac `s'` >> strip_tac >> fs[]
     >> `TYPE_SUBST s' in_x = TYPE_SUBST s' in_y` by (
-      (qspecl_then [`TYPE_SUBST sigma x`,`p`,`s'`,`in_x`] mp_tac) subtype_at_TYPE_SUBST
-      >> (qspecl_then [`TYPE_SUBST sigma y`,`p`,`s'`,`in_y`] mp_tac) subtype_at_TYPE_SUBST
-      >> rw[]
+      drule_then (qspec_then `s'` assume_tac) subtype_at_TYPE_SUBST
+      >> rev_drule_then (qspec_then `s'` assume_tac) subtype_at_TYPE_SUBST
+      >> ntac 2 $ first_x_assum $ drule_then strip_assume_tac
+      >> gs[FORALL_AND_THM,IMP_CONJ_THM]
     )
-    >> unabbrev_all_tac
     >> `TYPE_SUBST ((ty,Tyvar a)::MAP (TYPE_SUBST [(ty,Tyvar a)] ## I) sigma)
       = TYPE_SUBST [(ty,Tyvar a)] o TYPE_SUBST sigma` by (
       rw[FUN_EQ_THM,TYPE_SUBST_compose,TYPE_SUBST_tyvars]
-      >> match_mp_tac REV_ASSOCD_reorder
+      >> irule REV_ASSOCD_reorder
       >> rw[ALL_DISTINCT,MAP_MAP_o]
       >- fs[o_PAIR_MAP,ALL_DISTINCT_APPEND]
       >- (
-        qpat_x_assum `!x. MEM _ (tyvars (Tyvar a)) \/ _ ==> ~MEM _ _` (qspec_then `a` mp_tac)
-        >> unabbrev_all_tac
+        unabbrev_all_tac
+        >> qpat_x_assum `!x. MEM _ (tyvars (Tyvar a)) \/ _ ==> ~MEM _ _` $ qspec_then `a` mp_tac
         >> rw[MEM_MAP,tyvars_def]
       )
       >- fs[o_PAIR_MAP]
-      >> CONV_TAC(RHS_CONV(PURE_ONCE_REWRITE_CONV [INSERT_SING_UNION]))
+      >> CONV_TAC $ RHS_CONV $ PURE_ONCE_REWRITE_CONV [INSERT_SING_UNION]
       >> fs[AC UNION_ASSOC UNION_COMM]
     )
     >> unabbrev_all_tac
-    >> rw[]
-    >> assume_tac TYPE_SUBST_eating
-    >> fs[FUN_EQ_THM]
+    >> (dxrule_then assume_tac TYPE_SUBST_eating
+      ORELSE
+        dxrule_then assume_tac $
+          CONV_RULE (ONCE_DEPTH_CONV $ LAND_CONV SYM_CONV) TYPE_SUBST_eating)
+    >> gs[FUN_EQ_THM]
+  )
+  >> conj_asm1_tac
+  >- (
+    rw[EVERY_MEM,MEM_MAP]
+    >> fs[unify_types_invariant_def,ELIM_UNCURRY]
+    >> rename[`MEM y sigma`]
+    >> PairCases_on `y`
+    >> drule_then assume_tac $ Q.ISPEC `SND` MEM_MAP_f
+    >> qpat_x_assum `!x. _ ==> ?y. _` $ drule_then strip_assume_tac
+    >> qpat_x_assum `EVERY _ _` (fn x =>
+      drule_then strip_assume_tac $ SIMP_RULE std_ss [EVERY_MEM] x
+      >> drule_then strip_assume_tac $ SIMP_RULE std_ss [EVERY_MEM,Once subtype_at_eq] x
+    )
+    >> qpat_x_assum `!x. MEM x $ MAP SND sigma ==> _` $ drule_then strip_assume_tac
+    >> gvs[] >> Cases_on `y0` >> rw[TYPE_SUBST_def,REV_ASSOCD_def]
+  )
+  (* idempotent *)
+  >- (
+    fs[idempotent_thm,unify_types_invariant_def,clean_tysubst_id]
+    >> `clean_tysubst sigma = sigma` by (
+      irule clean_tysubst_id >> rw[]
+      >> fs[GSYM EVERY_MEM]
+      >> qpat_x_assum `EVERY _ $ MAP SND _` $ mp_tac o REWRITE_RULE[EVERY_MAP]
+      >> match_mp_tac EVERY_MONOTONIC
+      >> fs[ELIM_UNCURRY]
+    )
+    >> pop_assum $ fs o single
+    >> dep_rewrite.DEP_REWRITE_TAC[clean_tysubst_id]
+    >> conj_asm1_tac
+    >- (
+      fs[ALL_DISTINCT,MAP_MAP_o,o_DEF,ETA_THM,EVERY_MAP,GSYM EVERY_MEM]
+      >> spose_not_then $ strip_assume_tac o REWRITE_RULE[MEM_MAP]
+      >> fs[EVERY_MEM] >> res_tac >> gs[]
+    )
+    >> dsimp[MEM_FLAT,MEM_MAP] >> CCONTR_TAC >> fs[]
+    >- (
+      fs[tyvars_TYPE_SUBST,REV_ASSOCD_def]
+      >> FULL_CASE_TAC >> fs[tyvars_def]
+    )
+    >- (
+      dxrule_then assume_tac $ Q.ISPEC `SND` MEM_MAP_f
+      >> fs[DISJ_IMP_THM,FORALL_AND_THM]
+      >> res_tac
+      >> gs[]
+    )
+    >- (
+      fs[tyvars_TYPE_SUBST,REV_ASSOCD_def]
+      >> FULL_CASE_TAC >> fs[]
+      >- (
+        imp_res_tac $ Q.ISPEC `SND` MEM_MAP_f
+        >> gvs[FORALL_AND_THM,DISJ_IMP_THM]
+        >> res_tac
+        >> gvs[]
+      )
+      >> rename[`MEM x $ tyvars $ Tyvar x'`,`Tyvar x = SND yy`]
+      >> PairCases_on `yy`
+      >> imp_res_tac $ Q.ISPEC `SND` MEM_MAP_f
+      >> imp_res_tac $ Q.ISPEC `FST` MEM_MAP_f
+      >> gvs[tyvars_def]
+      >> qpat_x_assum `!x. MEM (Tyvar x) $ MAP SND sigma ==> _` drule
+      >> rw[PULL_EXISTS,MEM_FLAT,MEM_MAP]
+      >> rpt $ goal_assum drule
+    )
   )
 QED
 
@@ -7918,11 +8053,12 @@ QED
 Theorem unify_types_invariant_init:
   !orig_l. unify_types_invariant orig_l orig_l []
 Proof
-  simp[unify_types_invariant_def] \\ rw[]
+  simp[unify_types_invariant_def,idempotent_NIL] \\ rw[]
   >- (fs[LIST_REL_EVERY_ZIP,EVERY_MEM,ZIP_MAP,MEM_MAP] \\ Cases \\ rw[]
   \\ Cases_on `x` \\ fs[equal_upto_rules])
   >- (asm_exists_tac >> qexists_tac `[]` >> fs[subtype_at_def])
-  >> rpt(qexists_tac `[]` >> rw[])
+  >> qmatch_asmsub_abbrev_tac `TYPE_SUBST s`
+  >> qexists_tac `s` >> fs[]
 QED
 
 Theorem unify_types_IMP_invariant:
@@ -7945,13 +8081,10 @@ Theorem unify_types_sound_list:
        ==> EVERY (λ(ty1,ty2). TYPE_SUBST sigma ty1 = TYPE_SUBST sigma ty2) l
 Proof
   rpt strip_tac
-  >> (qspecl_then [`sigma`,`Tyapp a (MAP FST l)`,`Tyapp a (MAP SND l)`] assume_tac) unify_types_sound
-  >> fs[unify_types_def]
+  >> qspecl_then [`sigma`,`Tyapp a (MAP FST l)`,`Tyapp a (MAP SND l)`] assume_tac unify_types_sound
+  >> fs[unify_types_def,EVERY_MEM,ELIM_UNCURRY]
   >> FULL_CASE_TAC
-  >- fs[MAP_EQ_f,EVERY_MEM,ELIM_UNCURRY]
-  >> fs[MAP_EQ_EVERY2,LIST_REL_EVERY_ZIP,ZIP_MAP]
-  >> fs[LAMBDA_PROD,MAP_MAP_o,o_DEF]
-  >> fs[EVERY_MAP,ELIM_UNCURRY]
+  >> gs[MAP_EQ_f,MAP_EQ_EVERY2,LIST_REL_EVERY_ZIP,ZIP_MAP,EVERY_MAP,MAP_MAP_o,o_DEF,EVERY_MEM,ELIM_UNCURRY]
 QED
 
 Theorem unify_types_complete_cyclic_non_unifiable:
@@ -7974,7 +8107,7 @@ Proof
   `type_size(TYPE_SUBST s (Tyvar a)) = type_size(TYPE_SUBST s ty)`
     by rw[] >>
   pop_assum mp_tac >>
-  rpt(pop_assum kall_tac) >>
+  rpt $ pop_assum kall_tac >>
   rw[]
 QED
 
@@ -7989,163 +8122,132 @@ Proof
   >> rw[LENGTH_MAP]
 QED
 
+Theorem unify_types_invariant_Tyapp:
+  unify_types_invariant [(ty1,ty2)] ((Tyapp a atys,Tyapp b btys)::l) sigma
+  /\ TYPE_SUBST θ (TYPE_SUBST sigma ty1) = TYPE_SUBST θ (TYPE_SUBST sigma ty2)
+  ==> TYPE_SUBST θ (Tyapp a atys) = TYPE_SUBST θ (Tyapp b btys)
+Proof
+  rw[Excl"TYPE_SUBST_def",unify_types_invariant_def,FORALL_AND_THM,DISJ_IMP_THM,AND_IMP_INTRO]
+  >> qmatch_asmsub_abbrev_tac `subtype_at (TYPE_SUBST _ ty1) p = SOME in_ty1`
+  >> qmatch_asmsub_abbrev_tac `subtype_at (TYPE_SUBST _ ty2) p = SOME in_ty2`
+  >> qmatch_asmsub_abbrev_tac `TYPE_SUBST θ (TYPE_SUBST sigma _)`
+  >> drule_then (qspec_then `θ` assume_tac) subtype_at_TYPE_SUBST
+  >> rev_drule_then (qspec_then `θ` assume_tac) subtype_at_TYPE_SUBST
+  >> dxrule_then assume_tac $ cj 1 $ REWRITE_RULE[EQ_IMP_THM] subtype_at_eq
+  >> gs[]
+QED
+
 Theorem unify_types_complete_step[local]:
   !l sigma ty1 ty2.
   unify_types_invariant [(ty1,ty2)] l sigma
   /\ unifiable (TYPE_SUBST sigma ty1) (TYPE_SUBST sigma ty2)
-  ==> IS_SOME (unify_types l sigma)
+  ==> ?s. unify_types l sigma = SOME s /\ idempotent s
+    /\ clean_tysubst s = s
 Proof
   ho_match_mp_tac unify_types_ind
   >> strip_tac
-  >- rw[unify_types_invariant_def,unify_types_def]
+  >- (
+    rw[unify_types_invariant_def,unify_types_def,idempotent_NIL]
+    >> fs[clean_tysubst_id,GSYM EVERY_MEM,EVERY_MAP]
+  )
   >> strip_tac
   >- (
     rw[unify_types_def]
-    >- (
-      first_x_assum match_mp_tac
-      >> qexists_tac `ty1`
-      >> qexists_tac `ty2`
-      >> fs[unify_types_invariant_def,equal_upto_eq]
-      >> asm_exists_tac
-      >> fs[]
+    >> qmatch_assum_abbrev_tac `unify_types_invariant _ ((Tyapp a atys,Tyapp b btys)::_) _`
+    >> `a = b /\ LENGTH atys = LENGTH btys` by (
+      gs[unifiable_def]
+      >> drule_all $ unify_types_invariant_Tyapp
+      >> fs[TYPE_SUBST_def,LIST_EQ_REWRITE]
     )
-    >- (
-      rfs[]
-      >> first_x_assum match_mp_tac
-      >> qexists_tac `ty1`
-      >> qexists_tac `ty2`
-      >> fs[]
-      >> match_mp_tac (GEN_ALL unify_types_invariant_pres2)
-      >> asm_exists_tac
-      >> fs[]
-    )
-    >> CCONTR_TAC
     >> fs[]
-    >> (
-      fs[unifiable_def,unify_types_invariant_def]
-      >> first_x_assum (qspecl_then [`Tyapp a atys`,`Tyapp b btys`] assume_tac)
-      >> fs[]
-      >> qmatch_assum_abbrev_tac `subtype_at (TYPE_SUBST _ ty1) _ = SOME in_ty1`
-      >> qmatch_assum_abbrev_tac `subtype_at (TYPE_SUBST _ ty2) _ = SOME in_ty2`
-      >> imp_res_tac subtype_at_TYPE_SUBST
-      >> NTAC 2 (first_x_assum (qspec_then `s` assume_tac))
-      >> rfs[]
-      >> imp_res_tac unify_types_complete_arity_non_unifiable
-      >> TRY ((first_x_assum (qspecl_then [`s`,`btys`,`atys`] assume_tac))
-        ORELSE (first_x_assum (qspecl_then [`s`,`b`,`a`] assume_tac)))
-      >> unabbrev_all_tac
-      >> fs[]
-      >> fs[]
+    >- (
+      first_x_assum irule
+      >> drule_then (irule_at Any) unify_types_invariant_pres1 >> fs[]
+    )
+    >- (
+      first_x_assum irule
+      >> drule_then (irule_at Any) unify_types_invariant_pres2 >> fs[]
     )
   )
   >> strip_tac
   >- (
     rpt strip_tac
-    >> first_x_assum (qspecl_then [`ty1`,`ty2`] assume_tac)
-    >> imp_res_tac unify_types_invariant_pres3
-    >> fs[unify_types_def]
+    >> dxrule_then assume_tac unify_types_invariant_pres3
+    >> first_x_assum dxrule_all >> fs[unify_types_def]
   )
-  >> (
-    rw[unify_types_def]
-    >- (
-      first_x_assum match_mp_tac
-      >> qexists_tac `ty1`
-      >> qexists_tac `ty2`
-      >> fs[unify_types_invariant_def,equal_upto_eq]
-      >> asm_exists_tac
-      >> fs[]
-    )
-    >- (
-      imp_res_tac unify_types_complete_cyclic_non_unifiable
-      >> CCONTR_TAC
-      >> fs[unifiable_def,unify_types_invariant_def,tyvars_def]
-      >> qpat_x_assum `!x. (_ = _) \/ _ ==> _` (qspec_then `a` assume_tac)
-      >> fs[]
-      >> NTAC 2 (
-        qmatch_assum_abbrev_tac `MEM a (tyvars ty_a)`
-        >> qmatch_assum_abbrev_tac `TYPE_SUBST _ (_ _ ty_a) = TYPE_SUBST _ (_ _ ty_ty)`
-          ORELSE qmatch_assum_abbrev_tac `TYPE_SUBST _ (_ _ ty_ty) = TYPE_SUBST _ (_ _ ty_a)`
-        >> first_x_assum (qspecl_then [`Tyvar a`,`ty`] assume_tac)
-        >> fs[]
-        >> imp_res_tac subtype_at_TYPE_SUBST
-        >> NTAC 2 (first_x_assum (qspec_then `s'` assume_tac))
-        >> rfs[]
-      )
-    )
-    >> drule(GEN_ALL unify_types_invariant_pres5)
-    >> rw[]
-    >> first_x_assum match_mp_tac
-    >> asm_exists_tac
-    >> rw[]
-    >> qpat_x_assum `unify_types_invariant _ (MAP _ _) _` kall_tac
-    >> fs[unifiable_def,unify_types_invariant_def,tyvars_def]
-    >> qmatch_goalsub_abbrev_tac `TYPE_SUBST ts ty1`
-    >> qpat_x_assum `!x. (_ = _) \/ _ ==> _` (qspec_then `a` assume_tac)
-    >> fs[]
+  >> rw[unify_types_def]
+  >- (
+    first_x_assum irule
+    >> rpt $ goal_assum $ drule_at Any
+    >> fs[unify_types_invariant_def,equal_upto_eq]
+  )
+  >- (
+    drule_at Any unify_types_complete_cyclic_non_unifiable
+    >> CCONTR_TAC
+    >> fs[unifiable_def,unify_types_invariant_def,tyvars_def,FORALL_AND_THM,DISJ_IMP_THM]
     >> NTAC 2 (
       qmatch_assum_abbrev_tac `MEM a (tyvars ty_a)`
       >> qmatch_assum_abbrev_tac `TYPE_SUBST _ (_ _ ty_a) = TYPE_SUBST _ (_ _ ty_ty)`
         ORELSE qmatch_assum_abbrev_tac `TYPE_SUBST _ (_ _ ty_ty) = TYPE_SUBST _ (_ _ ty_a)`
-      >> first_x_assum (qspecl_then [`Tyvar a`,`ty`] assume_tac)
-      >> fs[]
-      >> NTAC 2 (
-        imp_res_tac subtype_at_TYPE_SUBST
-        >> NTAC 2 (first_x_assum (qspec_then `s` assume_tac))
-        >> `TYPE_SUBST s ty = TYPE_SUBST s (Tyvar a)` by rfs[]
-        >> imp_res_tac TYPE_SUBST_eating
-        >> `TYPE_SUBST ((ty,Tyvar a)::MAP (TYPE_SUBST [(ty,Tyvar a)] ## I) sigma)
-          = TYPE_SUBST [(ty,Tyvar a)] o TYPE_SUBST sigma` by (
-          rw[FUN_EQ_THM,TYPE_SUBST_compose,TYPE_SUBST_tyvars]
-          >> match_mp_tac REV_ASSOCD_reorder
-          >> rw[ALL_DISTINCT,MAP_MAP_o]
-          >- fs[o_PAIR_MAP,ALL_DISTINCT_APPEND]
-          >- (
-            qpat_x_assum `!x. (_ = _) \/ _ ==> ~MEM _ _` (qspec_then `a` mp_tac)
-            >> unabbrev_all_tac
-            >> rw[MEM_MAP,tyvars_def]
-            >- (
-              Cases_on `Tyvar a = SND y` >> rw[]
-              >> first_x_assum (qspec_then `y'` mp_tac)
-              >> rw[]
-              >- (DISJ1_TAC >> Cases_on `y'` >> Cases_on `y` >> fs[PAIR_MAP_THM])
-              >> fs[]
-            )
-            >> rw[MAP_MAP_o,o_PAIR_MAP]
-          )
-          >> unabbrev_all_tac
-          >> fs[AC UNION_ASSOC UNION_COMM]
-          >> CONV_TAC(RHS_CONV(PURE_ONCE_REWRITE_CONV [INSERT_SING_UNION]))
-          >> fs[]
-        )
-        >> unabbrev_all_tac
-        >> rfs[FUN_EQ_THM]
-        >> pop_assum kall_tac
-        >> qexists_tac `s`
-        >> fs[]
-      )
+      >> drule_then (qspec_then `s` assume_tac) subtype_at_TYPE_SUBST
+      >> rev_drule_then (qspec_then `s` assume_tac) subtype_at_TYPE_SUBST
+      >> rfs[GSYM TYPE_SUBST_def,Excl"TYPE_SUBST_def"]
     )
+  )
+  >> drule unify_types_invariant_pres5 >> rw[]
+  >> first_x_assum $ dxrule_at_then Any irule
+  >> fs[unifiable_def,unify_types_invariant_def,tyvars_def,DISJ_IMP_THM,FORALL_AND_THM]
+  >> qmatch_goalsub_abbrev_tac `TYPE_SUBST ts ty1`
+  >> NTAC 4 (
+    qmatch_assum_abbrev_tac `MEM a (tyvars ty_a)`
+    >> qmatch_assum_abbrev_tac `TYPE_SUBST s (_ _ ty_a) = TYPE_SUBST _ (_ _ ty_ty)`
+      ORELSE qmatch_assum_abbrev_tac `TYPE_SUBST s (_ _ ty_ty) = TYPE_SUBST _ (_ _ ty_a)`
     >> qexists_tac `s`
+    >> drule_then (qspec_then `s` assume_tac) subtype_at_TYPE_SUBST
+    >> rev_drule_then (qspec_then `s` assume_tac) subtype_at_TYPE_SUBST
+    >> `TYPE_SUBST s ty = TYPE_SUBST s (Tyvar a)` by rfs[]
+    >> drule_then assume_tac TYPE_SUBST_eating
+    >> `TYPE_SUBST ((ty,Tyvar a)::MAP (TYPE_SUBST [(ty,Tyvar a)] ## I) sigma)
+      = TYPE_SUBST [(ty,Tyvar a)] o TYPE_SUBST sigma` by (
+      rw[FUN_EQ_THM,TYPE_SUBST_compose,TYPE_SUBST_tyvars]
+      >> irule REV_ASSOCD_reorder
+      >> unabbrev_all_tac
+      >> fs[ALL_DISTINCT,MAP_MAP_o,o_PAIR_MAP,ALL_DISTINCT_APPEND]
+      >> CONV_TAC $ RHS_CONV $ ONCE_DEPTH_CONV $ REWR_CONV INSERT_SING_UNION
+      >> fs[AC UNION_ASSOC UNION_COMM]
+    )
     >> unabbrev_all_tac
     >> fs[FUN_EQ_THM]
   )
 QED
 
 Theorem unify_types_complete:
-  !ty1 ty2. unifiable ty1 ty2 = IS_SOME (unify_types [(ty1,ty2)] [])
+  !ty1 ty2. unifiable ty1 ty2 <=> IS_SOME $ unify_types [(ty1,ty2)] []
 Proof
-  rw[EQ_IMP_THM]
+  rw[EQ_IMP_THM,IS_SOME_EXISTS]
   >- (
-    match_mp_tac unify_types_complete_step
-    >> fs[TYPE_SUBST_NIL]
-    >> qexists_tac `ty1`
-    >> qexists_tac `ty2`
-    >> assume_tac unify_types_invariant_init
-    >> fs[]
+    qmatch_goalsub_abbrev_tac `unify_types l _`
+    >> qspec_then `l` assume_tac unify_types_invariant_init
+    >> qunabbrev_tac `l`
+    >> dxrule_then assume_tac unify_types_complete_step
+    >> gs[TYPE_SUBST_NIL]
   )
-  >> rw[is_instance_refl,ELIM_UNCURRY,unifiable_def]
-  >> qexists_tac `THE (unify_types [(ty1,ty2)] [])`
-  >> match_mp_tac unify_types_sound
-  >> fs[option_CLAUSES]
+  >> fs[unifiable_def]
+  >> drule_then (irule_at Any) unify_types_sound
+QED
+
+Theorem unify_types_props:
+  !s ty1 ty2. unify_types [(ty1,ty2)] [] = SOME s
+  ==> idempotent s /\ clean_tysubst s = s
+Proof
+  rpt gen_tac >> strip_tac
+  >> qmatch_asmsub_abbrev_tac `unify_types l _`
+  >> qspec_then `l` assume_tac unify_types_invariant_init
+  >> qunabbrev_tac `l`
+  >> dxrule unify_types_complete_step
+  >> impl_tac
+  >- (fs[TYPE_SUBST_NIL,unifiable_def] >> drule_then (irule_at Any) unify_types_sound)
+  >> fs[]
 QED
 
 Theorem unify_sound:
